[minor] Remove duplicated code from CodeTriples.

pico-ifc-coq/dyn_allocation/CodeSpecs.v
@@ -15,6 +15,7 @@ Require Import ConcreteMachine.
 Require Import Coq.Arith.Compare_dec.
 Require Import ConcreteExecutions.
 Require Import EquivDec.
+Require Import CodeTriples.
 
 Section CodeSpecs.
 Local Open Scope Z_scope.
@@ -30,311 +31,14 @@ Variable stamp_cblock : Mem.stamp cblock = Kernel.
 
 Notation cstep := (cstep cblock).
 Notation runsToEscape := (runsToEscape cblock).
+Notation HT := (HT cblock).
+Notation HTEscape := (HTEscape cblock).
 
 Definition imemory : Type := list Instr.
 Definition stack : Type := list CStkElmt.
 Definition code := list Instr.
 Definition state := CS.
-
-(* ---------------------------------------------------------------- *)
-(* Specs for self-contained code *)
-
-(* ================================================================ *)
-(* Hoare Triples *)
-
-(* Instruction memory contains code [c] starting at address [pc]. *)
-Fixpoint code_at (pc: Z) (im: imemory) (c: code): Prop :=
-  match c with
-  | nil     => True
-  | i :: c' => index_list_Z pc im = Some i 
-               /\ code_at (pc + 1) im c'
-  end.
-
-Lemma code_at_compose_1: forall im c1 c2 n,
-  code_at n im (c1 ++ c2) ->
-  code_at n im c1.
-Proof.
-  induction c1; intros; simpl in *.
-  intuition.
-  intuition. eapply IHc1. eauto.
-Qed.
-
-Lemma code_at_compose_2: forall im c1 c2 n,
-  code_at n im (c1 ++ c2) ->
-  code_at (n + Z_of_nat (length c1)) im c2.
-Proof.
-  induction c1; intros; simpl in *.
-
-  exact_f_equal H; omega.
-
-  intuition.
-  apply_f_equal IHc1; eauto; zify; omega.
-Qed.
-
-Lemma code_at_app : forall c2 c1 n, 
-  n = Z_of_nat (length c1) -> 
-  code_at n (c1 ++ c2) c2.
-Proof.
-  induction c2; intros. 
-  simpl. auto.
-  simpl. 
-  split. 
-  rewrite index_list_Z_app. auto.
-  subst n; auto.
-  replace (c1 ++ a :: c2) with ((c1 ++ [a]) ++ c2). 
-  eapply IHc2.
-  rewrite app_length. simpl. subst n; auto.
-  zify; omega. 
-  rewrite app_ass. auto.
-Qed.
-
-Lemma code_at_id : forall c, code_at 0%Z c c.
-Proof.
-  intros. pattern c at 1.  replace c with ([]++c) by auto.
-  eapply code_at_app. 
-  auto.
-Qed.
-  
 Definition HProp := memory -> stack -> Prop.
-
-(* Hoare triple for a list of instructions *)
-
-Definition HT (c: code) (P Q: HProp)
-:= forall imem stk0 mem0 fh n n',
-  code_at n fh c ->
-  P mem0 stk0 ->
-  n' = n + Z_of_nat (length c) -> 
-  exists stk1 mem1,
-  Q mem1 stk1 /\
-  runsToEnd cblock 
-             (CState mem0 fh imem stk0 (n, handlerTag) true)
-             (CState mem1 fh imem stk1 (n', handlerTag) true).
-
-Inductive Outcome :=
-| Success
-| Failure.
-
-Definition predicted_outcome (o: Outcome) raddr pc priv :=
-  match o with
-  | Success => priv = false /\ pc = raddr
-  | Failure => priv = true  /\ pc = (-1, handlerTag)
-  end.
-
-Definition HTEscape raddr
-  (c: code)
-  (P: memory -> stack -> Prop)
-  (Q: memory -> stack -> Prop * Outcome)
-:= forall imem stk0 mem0 fh n,
-  code_at n fh c ->
-  P mem0 stk0 ->
-  exists stk1 mem1 pc1 priv1,
-  let (prop, outcome) := Q mem1 stk1 in
-  prop /\
-  predicted_outcome outcome raddr pc1 priv1 /\
-  runsToEscape
-    (CState mem0 fh imem stk0 (n, handlerTag) true)
-    (CState mem1 fh imem stk1 pc1 priv1).
-
-Lemma HTEscape_strengthen_premise: forall r c (P' P: HProp) Q,
-  HTEscape r c P  Q ->
-  (forall m s, P' m s -> P m s) ->
-  HTEscape r c P' Q.
-Proof.
-  introv HTPQ P'__P.
-  unfold HTEscape; intros.
-  edestruct HTPQ as [mem2 [stk2 [HR RTE2]]]; eauto.
-Qed.
-
-Lemma HTEscape_compose: forall r c1 c2 P Q R,
-  HT         c1 P Q ->
-  HTEscape r c2 Q R ->
-  HTEscape r (c1 ++ c2) P R.
-Proof.
-  introv H_HT H_HTE.
-  intro; intros.
-
-  edestruct H_HT as [cache1 [stk1 [HQ Hstar1]]]; eauto.
-  eapply code_at_compose_1; eauto.
-
-  edestruct H_HTE as [stk2 [cache2 [pc2 [priv2 Hlet]]]]; eauto.
-  eapply code_at_compose_2; eauto.
-
-  exists stk2 cache2 pc2 priv2.
-  destruct (R cache2 stk2).
-  destruct Hlet as [? [Houtcome ?]].
-  destruct o; unfold predicted_outcome in Houtcome; simpl; intuition; subst.
-  - eapply rte_success.
-    eapply runsUntilUser_trans; eauto.
-    inv H2; eauto.
-    apply runsToEnd_r in STAR.
-    simpl in STAR. congruence.
-  - eapply rte_fail.
-    eapply runsToEnd_trans; eauto.
-    inv H2; eauto.
-    + apply runsUntilUser_r in STAR.
-      simpl in STAR. congruence.
-    + simpl. omega. 
-Qed.
-
-Lemma HTEscape_append: forall r c1 c2 P Q,
-  HTEscape r c1 P Q ->
-  HTEscape r (c1 ++ c2) P Q.
-Proof.
-  unfold HTEscape.
-  intros.
-  exploit code_at_compose_1; eauto.
-Qed.
-
-Lemma HT_compose: forall c1 c2 P Q R,
-  HT   c1 P Q ->
-  HT   c2 Q R ->
-  HT   (c1 ++ c2) P R.
-Proof.
-  unfold HT   in *.
-  intros c1 c2 P Q R HT1 HT2 imem stk0 mem0 fh0 n n' HC12 HP Hn'.
-  subst.
-  
-  edestruct HT1 as [stk1 [mem1 [HQ RTE1]]]; eauto.
-  apply code_at_compose_1 in HC12; eauto.
-
-  edestruct HT2 as [stk2 [mem2 [HR RTE2]]]; eauto.
-  apply code_at_compose_2 in HC12; eauto.
-
-  eexists. eexists. intuition. eauto.
-  replace (@nil CEvent) with (@nil CEvent++@nil CEvent) by reflexivity.
-  eapply runsToEnd_trans; eauto.
-
-  (* NC: why is this let-binding necessary ? *)
-  let t := (rewrite app_length; zify; omega) in
-  exact_f_equal RTE2; rec_f_equal t.
-  (* Because 'tacarg's which are not 'id's or 'term's need to be
-     preceded by 'ltac' and enclosed in parens.  E.g., the following
-     works:
-
-       exact_f_equal RTE2;
-       rec_f_equal ltac:(rewrite app_length; zify; omega).
-
-     See grammar at
-     http://coq.inria.fr/distrib/8.4/refman/Reference-Manual012.html
-
-   *)
-Qed.
-
-(* An alternate version, which works better when unifying pre-conditions *)
-Lemma HT_compose_flip : forall c1 c2 P Q R,
-                      HT c2 Q R ->
-                      HT c1 P Q ->
-                      HT (c1 ++ c2) P R.
-Proof. intros. eauto using HT_compose. Qed.
-
-(* ================================================================ *)
-(* Lemmas on Hoare Triples *)
-
-Lemma HT_strengthen_premise: forall c (P' P Q: HProp),
-  HT   c P  Q ->
-  (forall m s, P' m s -> P m s) ->
-  HT   c P' Q.
-Proof.
-  intros c P' P Q HTPQ P'__P.
-  intros imem stk0 c0 fh0 n n' Hcode HP' Hn'.
-  edestruct HTPQ as [mem2 [stk2 [HR RTE2]]]; eauto.
-Qed.
-
-Lemma HT_weaken_conclusion: forall c (P Q Q': HProp),
-  HT   c P  Q ->
-  (forall m s, Q m s -> Q' m s) ->
-  HT   c P Q'.
-Proof.
-  intros ? ? ? ? HTPQ ?.
-  intros imem stk0 c0 fh0 n n' Hcode HP' Hn'.
-  edestruct HTPQ as [stk2 [c2 [HR RTE2]]]; eauto.
-Qed.
-
-Lemma HT_consequence: forall c (P' P Q Q': HProp),
-  HT   c P Q ->
-  (forall m s, P' m s -> P m s) ->
-  (forall m s, Q m s -> Q' m s) ->
-  HT   c P' Q'.
-Proof.
-  intros.
-  eapply HT_weaken_conclusion; eauto.
-  eapply HT_strengthen_premise; eauto.
-Qed.
-
-(* A strengthened rule of consequence that takes into account that [Q]
-   need only be provable under the assumption that [P] is true for
-   *some* state.  This lets us utilize any "pure" content in [P] when
-   establishing [Q]. *)
-Lemma HT_consequence': forall c (P' P Q Q': HProp),
-  HT   c P Q ->
-  (forall m s, P' m s -> P m s) ->
-  (forall m s, (exists m' s', P' m' s') -> Q m s -> Q' m s) ->
-  HT   c P' Q'.
-Proof.
-  intros ? ? ? ? ? HTPQ HPP' HP'QQ'.
-  intros imem stk0 c0 fh0 n n' Hcode HP' Hn'.
-  edestruct HTPQ as [stk2 [c2 [HR RTE2]]]; eauto.
-  eexists. eexists. eexists.
-  intuition.
-  eapply HP'QQ'; eauto.
-  eauto.
-Qed.
-
-Lemma HT_decide_join: forall T (v: T) c c1 c2 P1 P2 P1' P2' Q (D: T -> Prop),
-  (HT   c1 P1 Q -> ~ D v -> HT   c P1' Q) ->
-  (HT   c2 P2 Q ->   D v -> HT   c P2' Q) ->
-  (forall v, ~ D v \/ D v) ->
-  HT   c1 P1 Q ->
-  HT   c2 P2 Q ->
-  (* Switched to implication here.  I think this is a weaker
-     assumption, and it's closer to the form of the [ifNZ] spec I want
-   *)
-  HT   c (fun m s => (~ D v -> P1' m s) /\ (D v -> P2' m s)) Q.
-Proof.
-  intros ? v c c1 c2 P1 P2 P1' P2' Q D spec1 spec2 decD HT1 HT2.
-  unfold HT. intros imem mem0 stk0 n n' H_code_at HP neq.
-  (* destruct HP as [v [[HDv HP1'] | [HnDv HP2']]]. *)
-  pose (decD v) as dec. intuition.
-Qed.
-
-(* Hoare triples are implications, and so this corresponds to the
-   quantifier juggling lemma:
-
-     (forall x, (P x -> Q)) ->
-     ((exists x, P x) -> Q)
-
-*)
-Lemma HT_forall_exists: forall T c P Q,
-  (forall (x:T), HT   c (P x) Q) ->
-  HT   c (fun m s => exists (x:T), P x m s) Q.
-Proof.
-  intros ? c P Q HPQ.
-  unfold HT.
-  intros imem stk0 c0 fh0 n n' Hcode_at [x HPx] neq.
-  eapply HPQ; eauto.
-Qed.
-
-(* The other direction (which I don't need) is provable from
-   [HT_strengthen_premise] *)
-Lemma HT_exists_forall: forall T c P Q,
-  HT   c (fun m s => exists (x:T), P x m s) Q ->
-  (forall (x:T), HT   c (P x) Q).
-Proof.
-  intros ? c P Q HPQ x.
-  eapply HT_strengthen_premise.
-  eapply HPQ.
-  intuition.
-  eauto.
-Qed.
-
-Lemma HT_fold_constant_premise: forall (C:Prop) c P Q ,
-  (C -> HT c P Q) ->
-  HT c (fun m s => C /\ P m s) Q.
-Proof.
-  unfold HT.
-  iauto.
-Qed.
-
 (* ================================================================ *)
 (* Specs for concrete code *)
 
@@ -350,7 +54,7 @@ Lemma add_spec: forall (z1 z2 z: val) (l1 l2: Z) (m: memory) (s: stack),
 Proof.
   (* Introduce hyps *)
   intros.
-  unfold HT. intros. intuition.
+  unfold CodeTriples.HT. intros. intuition.
   eexists.
   eexists.
   eexists.
@@ -372,7 +76,7 @@ Lemma sub_spec: forall z1 l1 z2 l2 z, forall m0 s0,
      (fun m s => m = m0 /\ s = (z1,l1) ::: (z2,l2) ::: s0)
      (fun m s => m = m0 /\ s = (z,handlerTag) ::: s0).
 Proof.
-  unfold HT; intros.
+  unfold CodeTriples.HT; intros.
   eexists.
   eexists.
   intuition.
@@ -548,7 +252,7 @@ Proof.
     + eapply push_spec'.
     + simpl.
 
-  unfold HT. intros. intuition.
+  unfold CodeTriples.HT. intros. intuition.
   destruct stk0; simpl in H2; inv H2.
   destruct stk0; simpl in H0; inv H0.
   simpl in *.
@@ -590,7 +294,7 @@ Lemma pop_spec: forall v vl, forall m0 s0,
      (fun m s => m = m0 /\ s = CData (v,vl) :: s0)
      (fun m s => m = m0 /\ s = s0).
 Proof.
-  unfold HT.
+  unfold CodeTriples.HT.
   intros.
   eexists.
   eexists.
@@ -610,7 +314,7 @@ Lemma nop_spec: forall m0 s0,
      (fun m s => m = m0 /\ s = s0)
      (fun m s => m = m0 /\ s = s0).
 Proof.
-  unfold HT.
+  unfold CodeTriples.HT.
   intros.
   exists s0.
   exists m0.
@@ -657,7 +361,7 @@ Lemma store_spec_wp: forall Q b a al v,
                    Q m s)
      Q.
 Proof.
-  unfold HT.
+  unfold CodeTriples.HT.
   intros.
   jauto_set_hyps; intros.
   eexists.
@@ -682,7 +386,7 @@ Lemma store_spec: forall b a al v vl m s,
      (fun m1 s1 => s1 = s /\
                    store b a (v,vl) m = Some m1).
 Proof.
-  unfold HT.
+  unfold CodeTriples.HT.
   intros.
   edestruct valid_store.
   iauto.
@@ -879,7 +583,7 @@ Lemma ifNZ_spec_helper: forall v l t f Pt Pf Q,
        Q.
 Proof.
   intros v l t f Pt Pf Q HTt HTf.
-  eapply HT_decide_join with (D := fun v => v = 0).
+  eapply HT_decide_join' with (D := fun v => v = 0).
   apply ifNZ_spec_NZ.
   apply ifNZ_spec_Z.
   intros; omega.
@@ -1042,10 +746,10 @@ Proof.
   exists s0.
   intuition; subst; auto.
 
-  apply (HT_consequence' _ _ _ _ _ Hb); intuition.
+  apply (HT_consequence' _ _ _ _ _ _ Hb); intuition.
   elimtype False; jauto.
 
-  apply (HT_consequence' _ _ _ _ _ Hcbs); intuition.
+  apply (HT_consequence' _ _ _ _ _ _ Hcbs); intuition.
   elimtype False; jauto.
 Qed.
 
@@ -1107,11 +811,11 @@ Proof.
   exists s0.
   intuition; subst; auto.
 
-  apply (HT_consequence' _ _ _ _ _ (Hb m0 s0)); intuition.
+  apply (HT_consequence' _ _ _ _ _ _ (Hb m0 s0)); intuition.
   elimtype False; jauto.
 
   fold cases.
-  apply (HT_consequence' _ _ _ _ _ (Hcbs m0 s0)); intuition.
+  apply (HT_consequence' _ _ _ _ _ _ (Hcbs m0 s0)); intuition.
   elimtype False; jauto.
 Qed.
 
@@ -1404,7 +1108,7 @@ Qed.
 Lemma nop_spec_wp: forall Q,
   HT [Noop] Q Q.
 Proof.
-  unfold HT; simpl; intros.
+  unfold CodeTriples.HT; simpl; intros.
   eexists; eexists; intuition eauto. subst.
 
   (* Run an instruction *)
@@ -1418,7 +1122,7 @@ Lemma ret_specEscape: forall raddr (P: HProp),
     (fun m s => (P m s , Success)).
 Proof.
   intros. cases raddr; subst.
-  unfold HTEscape. intros. intuition.
+  unfold CodeTriples.HTEscape. intros. intuition.
   jauto_set_hyps; intuition.
   repeat eexists.
   eauto.
@@ -1440,7 +1144,7 @@ Lemma jump_specEscape_Failure: forall tag raddr (P: HProp),
            (fun m s => (P m s , Failure)).
 Proof.
   intros.
-  unfold HTEscape. intros.
+  unfold CodeTriples.HTEscape. intros.
   jauto_set_hyps; intuition.
   repeat eexists.
   eauto.
